- Added rm -f coq/*.{glob,vo,vok} to make clean - Changed eq to eqb - Removed boolean comparators of values outside of resp module - Moved tests to separate file - Created FLAGS module

coq/coqcaptest.ml
@@ -27,7 +27,8 @@ open Morello
 
 module M = struct
   include MorelloCapabilityWithStrfcap
-
+  include TestCaps
+  
   let cap_1 : t = TestCaps.c1
   let cap_1_bytes = TestCaps.c1_bytes
   let cap_2 : t = TestCaps.c2
