coq/Utils.v
@@ -245,6 +245,14 @@ Definition float_of_bits (_:Z): float := PrimFloat.zero. (* TODO: implement *)
 
 Definition bits_of_float (_:float) : Z := Z.zero. (* TODO: implement *)
 
+Fixpoint List_bool_eqb (l1:list bool) (l2:list bool) : bool := 
+  match (l1,l2) with
+    ([],[]) => true 
+  | ([],_) => false 
+  | (_,[]) => false 
+  | (h1::t1,h2::t2) => (Bool.eqb h1 h2) && List_bool_eqb t1 t2
+  end.
+
 Definition string_of_bool (b:bool) :=
   match b with
   | true => "true"
