Makefile
@@ -244,6 +244,7 @@ clean-sibylfs-src:
 
 .PHONY: clean
 clean:
+	$(Q)rm -f coq/*.{glob,vo,vok}
 	$(Q)rm -f webcerb.concrete webcerb.symbolic cerberus-webserver
 	$(Q)rm -f $(LIBC_TARGETS)
 	$(Q)dune clean
